Exercise 3

teaching/taltech2018/ex/ex3/RefinedStack.fst
@@ -30,21 +30,3 @@ module RefinedStack
           of stacks in `RefinedStack.fsti` and give proofs of these properties in the current file.
 
 *)
-
-let stack = list int
-
-let is_empty s = Nil? s
-
-let empty = []
-
-let push i s = i::s
-
-let pop (i::s) = s
-
-let top (i::s) = i
-
-let lemma_push_top s i = ()
-
-let lemma_push_pop s i = ()
-
-let lemma_top_pop_push s = ()
