teaching/taltech2018/sols_hidden/ex3/RefinedStack.fsti
@@ -1,12 +1,23 @@
 module RefinedStack
 
-val stack : Type0  (* type of stacks *)
+(*
+
+  Exercise 3.
+
+  See `RefinedStack.fst` for details.
+
+*)
+
+val stack : Type0
 
 val is_empty : stack -> GTot bool
+
 val empty : s:stack{is_empty s}
 
 val push : int -> stack -> s:stack{~(is_empty s)}
+
 val pop : s:stack{~(is_empty s)} -> stack           
+
 val top : s:stack{~(is_empty s)} -> int
 
 val lemma_push_top : s:stack -> i:int -> 
